Some progress on inst selection

compiler1/proofs/word_instProofScript.sml
@@ -6,7 +6,7 @@ val _ = new_theory "word_instProof";
 
 val sym_sub_tac = SUBST_ALL_TAC o SYM;
 
-(*First step: Make expressions have ≤ 2 args*)
+(*First step: Make op expressions have exactly 2 args*)
 (*Semantics*)
 val flatten_exp_ok = prove(``
   ∀exp s.
@@ -19,14 +19,14 @@ val flatten_exp_ok = prove(``
       (match_mp_tac LIST_EQ>>unabbrev_all_tac>>fs[EL_MAP,EL_MEM])>>
     metis_tac[])
   >>
-    fs[word_exp_def,LET_THM]>>IF_CASES_TAC>>fs[word_op_def]>>
+    fs[word_exp_def,LET_THM,word_op_def]>>IF_CASES_TAC>>fs[]>>
     TRY(first_x_assum(qspec_then `s` assume_tac)>>rfs[]>>
     pop_assum sym_sub_tac>>fs[])>>metis_tac[option_CLAUSES])
 
 (*All ops are 2 args. Technically, we should probably check that Sub has 2 args. However, the semantics already checks that*)
 val binary_branch_exp_def = tDefine "binary_branch_exp" `
   (binary_branch_exp (Op Sub exps) = EVERY (binary_branch_exp) exps) ∧ 
-  (binary_branch_exp (Op op xs) = (LENGTH xs ≤ 2 ∧ EVERY (binary_branch_exp) xs)) ∧
+  (binary_branch_exp (Op op xs) = (LENGTH xs = 2 ∧ EVERY (binary_branch_exp) xs)) ∧
   (binary_branch_exp (Load exp) = binary_branch_exp exp) ∧ 
   (binary_branch_exp (Shift shift exp nexp) = binary_branch_exp exp) ∧  
   (binary_branch_exp exp = T)`
@@ -42,205 +42,31 @@ val flatten_exp_binary_branch_exp = prove(``
   binary_branch_exp (flatten_exp exp)``,
   ho_match_mp_tac flatten_exp_ind>>fs[flatten_exp_def,binary_branch_exp_def,EVERY_MEM,EVERY_MAP])
 
-val distinct_tar_reg_def = Define`
-  (distinct_tar_reg (Inst (Arith (Binop bop r1 r2 ri))) 
-    ⇔ (r1 ≠ r2 ∧ case ri of (Reg r3) => r1 ≠ r3 | _ => T)) ∧ 
-  (distinct_tar_reg (Inst (Arith (Shift l r1 r2 n)))
-    ⇔ r1 ≠ r2) ∧ 
-  (distinct_tar_reg (Seq p1 p2)
-    ⇔ (distinct_tar_reg p1 ∧ distinct_tar_reg p2)) ∧ 
-  (distinct_tar_reg (If cmp r1 ri c1 c2)
-    ⇔ (distinct_tar_reg c1 ∧ distinct_tar_reg c2)) ∧ 
-  (distinct_tar_reg (Call ret dest args handler)
-    ⇔ ((case ret of 
-        NONE => T
-      | SOME (n,names,ret_handler,l1,l2) => distinct_tar_reg ret_handler) ∧ 
-      (case handler of
-        NONE => T
-      | SOME (n,h,l1,l2) => distinct_tar_reg h))) ∧ 
-  (distinct_tar_reg prog = T)`
+val num_exp_equiv = prove(``
+  word_inst$num_exp = wordSem$num_exp``,
+  fs[FUN_EQ_THM]>>Induct>>
+  fs[wordSemTheory.num_exp_def,word_instTheory.num_exp_def])
 
-(*Instructions are 2 register code for arith ok*)
-val two_reg_insts_def = Define`
-  (two_reg_insts (Inst (Arith (Binop bop r1 r2 ri))) 
-    ⇔ (r1 = r2)) ∧ 
-  (two_reg_insts (Inst (Arith (Shift l r1 r2 n)))
-    ⇔ (r1 = r2)) ∧ 
-  (two_reg_insts (Seq p1 p2)
-    ⇔ (two_reg_insts p1 ∧ two_reg_insts p2)) ∧ 
-  (two_reg_insts (If cmp r1 ri c1 c2)
-    ⇔ (two_reg_insts c1 ∧ two_reg_insts c2)) ∧ 
-  (two_reg_insts (Call ret dest args handler)
-    ⇔ ((case ret of 
-        NONE => T
-      | SOME (n,names,ret_handler,l1,l2) => two_reg_insts ret_handler) ∧ 
-      (case handler of
-        NONE => T
-      | SOME (n,h,l1,l2) => two_reg_insts h))) ∧ 
-  (two_reg_insts prog = T)`
-
-(*TODO: move to HOL*)
-val insert_shadow = prove(``
-  ∀t a b c.
-  insert a b (insert a c t) = insert a b t``,
-  completeInduct_on`a`>>
-  Induct>>
-  simp[Once insert_def]>>
-  rw[]>>
-  simp[Once insert_def]>>
-  simp[Once insert_def,SimpRHS]>>
-  `(a-1) DIV 2 < a` by 
-    (`0 < (2:num)` by fs[] >>
-    imp_res_tac DIV_LT_X>>
-    first_x_assum match_mp_tac>>
-    DECIDE_TAC)>>
-  metis_tac[])
-
-val alist_insert_wf = prove(``
-  ∀a b s.
-  wf s ⇒ 
-  wf(alist_insert a b s)``,
-  ho_match_mp_tac alist_insert_ind>>rw[alist_insert_def]>>
-  metis_tac[wf_insert])
-
-val red_tac = 
-  EVERY_CASE_TAC>>
-  fs[get_vars_def,set_vars_def,state_component_equality,set_var_def,set_store_def,mem_store_def,call_env_def,fromList2_def,dec_clock_def]>>
-  metis_tac[alist_insert_wf,wf_insert,wf_def]
-
-val wf_preservation = prove(``
-  ∀prog s res s'.
-  wf s.locals ∧  
-  evaluate(prog,s) = (res,s')
-  ⇒ 
-  wf s'.locals``,
-  completeInduct_on`prog_size (K 0) prog`>>
-  rpt strip_tac>>
-  Cases_on`prog`>>
-  fs[evaluate_def,LET_THM,state_component_equality]
-  >-
-    red_tac
-  >-
-    (Cases_on`i`>>fs[inst_def,assign_def]>>
-    red_tac)
-  >-
-    red_tac
-  >-
-    red_tac
-  >-
-    red_tac
-  >-
-    red_tac
-  >-
-    cheat
-  >-
-    (fs[PULL_FORALL,AND_IMP_INTRO]>>
-    Cases_on`evaluate(p,s)`>>fs[]>>
-    res_tac>>fs[prog_size_def]>>pop_assum mp_tac>>discharge_hyps>-DECIDE_TAC>>
-    Cases_on`q=NONE`>>fs[]>>rw[]>>
-    res_tac>>
-    pop_assum kall_tac >> pop_assum mp_tac >> discharge_hyps>-DECIDE_TAC >>
-    metis_tac[])
-  >-
-    (EVERY_CASE_TAC>>
-    fs[PULL_FORALL,AND_IMP_INTRO,prog_size_def]>>
-    res_tac>>pop_assum mp_tac >> discharge_hyps>> TRY DECIDE_TAC>>metis_tac[])
-  >-
-    EVERY_CASE_TAC>>fs[alloc_def]>>
-    EVERY_CASE_TAC>>fs[gc_def,push_env_def,pop_env_def]
-
-    rpt (qpat_assum`A=SOME B` mp_tac)>>EVERY_CASE_TAC>>
-    LET_ELIM_TAC>>
-    fs[LET_THM,set_store_def]>>EVERY_CASE_TAC>>fs[state_component_equality]>>
-    metis_tac[wf_fromAList]   
-    EVERY_CASE_TAC>>fs[push_env
-
-    fs[set_store_def,push_env_def]>>
-     
-    IF_CASES_TAC>>
-    first_x_assum(qspec_then `p` mp_tac)>> 
-    discharge_hyps>-
-
-    discharge_hyps
-    cheat
-  >-
-    cheat
-  >-
-    cheat
-  >-
-    cheat
-  >-
-    red_tac
-)
-
- 
-(*Semantics preservation*)
-val three_to_two_reg_correct = prove(``
-  ∀prog s res s'.
-  distinct_tar_reg prog ∧ 
-  evaluate (prog,s) = (res,s') ∧ res ≠ SOME Error
-  ⇒ 
-  evaluate(three_to_two_reg prog,s) = (res,s')``,
-  ho_match_mp_tac three_to_two_reg_ind>>
-  rw[]>>fs[three_to_two_reg_def,evaluate_def,state_component_equality]>>
-  TRY
-    (ntac 2 (pop_assum mp_tac)>>fs[inst_def,assign_def,word_exp_def,get_vars_def,get_var_def,set_vars_def,alist_insert_def]>>
-    EVERY_CASE_TAC >>
-    fs[LET_THM,alist_insert_def,distinct_tar_reg_def,word_exp_def,lookup_insert,set_var_def,insert_shadow]>>NO_TAC)
-  >-
-    (ntac 2 (pop_assum mp_tac)>>LET_ELIM_TAC>>fs[distinct_tar_reg_def]>>
-    Cases_on`res'' = SOME Error`>>fs[]>>res_tac>>
-    EVERY_CASE_TAC>>fs[]>>
-    metis_tac[])
-  >-
-    (ntac 2 (pop_assum mp_tac)>>LET_ELIM_TAC>>fs[distinct_tar_reg_def]>>
-    unabbrev_all_tac>>
-    Cases_on`ret`>>Cases_on`handler`>>fs[evaluate_def]
-    >-
-      (EVERY_CASE_TAC>>fs[])
-    >-
-      (EVERY_CASE_TAC>>fs[]>>
-      res_tac>>fs[]>>
-      rfs[])
-    >>
-      PairCases_on`x`>>PairCases_on`x'`>>fs[]>>
-      Cases_on`get_vars args s`>>fs[]>>
-      Cases_on`find_code dest x s.code`>>fs[]>>
-      Cases_on`x'`>>Cases_on`cut_env x1 s.locals`>>fs[]>>
-      IF_CASES_TAC>>fs[push_env_def,LET_THM]>>
-      EVERY_CASE_TAC>>fs[]>>
-      res_tac>>fs[]>>
-      rfs[]))
-
-(*Syntactic correctness*)
-val three_to_two_reg_syn = prove(``
-  ∀prog. two_reg_insts (three_to_two_reg prog)``,
-  ho_match_mp_tac three_to_two_reg_ind>>rw[]>>fs[two_reg_insts_def,three_to_two_reg_def,LET_THM]>>EVERY_CASE_TAC>>fs[])
-
+(*2nd step: Convert expressions to insts*)
 val inst_select_exp_thm = prove(``
-  ∀s exp tar temp w.
-  word_exp s exp = SOME w ∧
-  (∀x. x ∈ domain s.locals ⇒ x < temp) ⇒ 
+  ∀tar temp exp s w.
+  binary_branch_exp exp ∧ 
+  word_exp s exp = SOME w ⇒ 
   let (res,s') = evaluate ((inst_select_exp tar temp exp),s) in
     res = NONE ∧
-    s' = s with locals:=s'.locals ∧ 
+    s' = s with locals:= s'.locals ∧ 
     ∀x. 
     if x = tar then lookup x s'.locals = SOME (Word w)
-    else 
-      x ∈ domain s.locals ⇒ (lookup x s.locals = lookup x s'.locals)``,
-  ho_match_mp_tac word_exp_ind>>rpt strip_tac>>
-  fs[LET_THM,inst_select_exp_def,evaluate_def,word_exp_def,inst_def,assign_def,set_var_def,lookup_insert,get_vars_def,set_vars_def,get_var_def]
+    else if x < temp then lookup x s'.locals = lookup x s.locals
+    else T``,
+  ho_match_mp_tac inst_select_exp_ind>>
+  rpt strip_tac>>
+  fs[LET_THM,inst_select_exp_def,evaluate_def,word_exp_def,inst_def,assign_def,set_var_def,lookup_insert,get_vars_def,set_vars_def,get_var_def,binary_branch_exp_def,binary_branch_exp_def]
+  >-(EVERY_CASE_TAC>>fs[alist_insert_def,lookup_insert])
+  >-(EVERY_CASE_TAC>>fs[alist_insert_def,lookup_insert])
   >-
-    (EVERY_CASE_TAC>>fs[alist_insert_def,lookup_insert])
-  >-
-    (EVERY_CASE_TAC>>fs[lookup_insert])
-  >-
-    (EVERY_CASE_TAC>>fs[]>>
-    first_x_assum(qspecl_then[`temp`,`temp+1`] mp_tac)>>
-    discharge_hyps_keep>-
-      (rw[]>>res_tac>>DECIDE_TAC)
-    >>
-    strip_tac>>fs[]>>
+    (EVERY_CASE_TAC>>fs[binary_branch_exp_def]>>
+    res_tac>>
     qpat_abbrev_tac`A = evaluate (B,C)`>>
     Cases_on`A`>>fs[]>>
     `lookup temp r.locals = SOME (Word x)` by metis_tac[]>>
@@ -249,24 +75,37 @@ val inst_select_exp_thm = prove(``
     rw[]>>first_x_assum(qspec_then `x'` assume_tac)>>
     `x' ≠ temp` by 
       (res_tac>>DECIDE_TAC)>>
+    `x' < temp+1` by DECIDE_TAC>>
     metis_tac[])
   >-
-    (*hard case where Op order optimizations come in*)
     cheat
-  >>
-    (EVERY_CASE_TAC>>fs[]>>
-    first_x_assum(qspecl_then[`temp`,`temp+1`] mp_tac)>>
-    discharge_hyps_keep>-
-      (rw[]>>res_tac>>DECIDE_TAC)
-    >>
-    strip_tac>>fs[]>>
+    (*Cases_on`op`>>fs[binary_branch_exp_def,IS_SOME_EXISTS]>>
+    EVERY_CASE_TAC>>res_tac>>
+    qpat_abbrev_tac`A=evaluate(B,C)`>>
+    Cases_on`A`>>fs[]>>
+    (*TODO: Strengthen IH so that this is true*)
+    `word_exp r exp' = SOME x'` by cheat>>
+    res_tac>>
+    qpat_abbrev_tac`A=evaluate(B,C)`>>
+    Cases_on`A`>>fs[]>>
+    cheat*)
+  >-
+    (EVERY_CASE_TAC>>fs[binary_branch_exp_def]>>
+    res_tac>>
     qpat_abbrev_tac`A = evaluate (B,C)`>>
     Cases_on`A`>>fs[]>>
     `lookup temp r.locals = SOME (Word x)` by metis_tac[]>>
-    fs[word_op_def,mem_load_def,state_component_equality,lookup_insert,Once num_exp_def]>>
-    (*Some weird type error??*)
-    cheat))
-
+    fs[word_op_def,mem_load_def,state_component_equality,lookup_insert,Once num_exp_def,num_exp_equiv]>>
+    rw[]>>Cases_on`x'=tar`>>fs[]>>
+    rw[]>>first_x_assum(qspec_then `x'` assume_tac)>>
+    `x' ≠ temp` by 
+      (res_tac>>DECIDE_TAC)>>
+    `x' < temp+1` by DECIDE_TAC>>
+    metis_tac[])
+  >>
+    Cases_on`v11`>>fs[binary_branch_exp_def,word_op_def])
+   
+(*
 val inst_select_thm = prove(``
   ∀prog st res rst temp.
   evaluate (prog,st) = (res,rst) ∧
@@ -322,7 +161,105 @@ val inst_select_thm = prove(``
   (*Induction -- IH must be strengthened so that temp 
     does not occur anywhere in the program as well*)
   >> cheat)
-    
+*)
+
+val distinct_tar_reg_def = Define`
+  (distinct_tar_reg (Inst (Arith (Binop bop r1 r2 ri))) 
+    ⇔ (r1 ≠ r2 ∧ case ri of (Reg r3) => r1 ≠ r3 | _ => T)) ∧ 
+  (distinct_tar_reg (Inst (Arith (Shift l r1 r2 n)))
+    ⇔ r1 ≠ r2) ∧ 
+  (distinct_tar_reg (Seq p1 p2)
+    ⇔ (distinct_tar_reg p1 ∧ distinct_tar_reg p2)) ∧ 
+  (distinct_tar_reg (If cmp r1 ri c1 c2)
+    ⇔ (distinct_tar_reg c1 ∧ distinct_tar_reg c2)) ∧ 
+  (distinct_tar_reg (Call ret dest args handler)
+    ⇔ ((case ret of 
+        NONE => T
+      | SOME (n,names,ret_handler,l1,l2) => distinct_tar_reg ret_handler) ∧ 
+      (case handler of
+        NONE => T
+      | SOME (n,h,l1,l2) => distinct_tar_reg h))) ∧ 
+  (distinct_tar_reg prog = T)`
+
+(*Instructions are 2 register code for arith ok*)
+val two_reg_insts_def = Define`
+  (two_reg_insts (Inst (Arith (Binop bop r1 r2 ri))) 
+    ⇔ (r1 = r2)) ∧ 
+  (two_reg_insts (Inst (Arith (Shift l r1 r2 n)))
+    ⇔ (r1 = r2)) ∧ 
+  (two_reg_insts (Seq p1 p2)
+    ⇔ (two_reg_insts p1 ∧ two_reg_insts p2)) ∧ 
+  (two_reg_insts (If cmp r1 ri c1 c2)
+    ⇔ (two_reg_insts c1 ∧ two_reg_insts c2)) ∧ 
+  (two_reg_insts (Call ret dest args handler)
+    ⇔ ((case ret of 
+        NONE => T
+      | SOME (n,names,ret_handler,l1,l2) => two_reg_insts ret_handler) ∧ 
+      (case handler of
+        NONE => T
+      | SOME (n,h,l1,l2) => two_reg_insts h))) ∧ 
+  (two_reg_insts prog = T)`
+
+(*TODO: move to HOL*)
+val insert_shadow = prove(``
+  ∀t a b c.
+  insert a b (insert a c t) = insert a b t``,
+  completeInduct_on`a`>>
+  Induct>>
+  simp[Once insert_def]>>
+  rw[]>>
+  simp[Once insert_def]>>
+  simp[Once insert_def,SimpRHS]>>
+  `(a-1) DIV 2 < a` by 
+    (`0 < (2:num)` by fs[] >>
+    imp_res_tac DIV_LT_X>>
+    first_x_assum match_mp_tac>>
+    DECIDE_TAC)>>
+  metis_tac[])
+ 
+(*Semantics preservation*)
+val three_to_two_reg_correct = prove(``
+  ∀prog s res s'.
+  distinct_tar_reg prog ∧ 
+  evaluate (prog,s) = (res,s') ∧ res ≠ SOME Error
+  ⇒ 
+  evaluate(three_to_two_reg prog,s) = (res,s')``,
+  ho_match_mp_tac three_to_two_reg_ind>>
+  rw[]>>fs[three_to_two_reg_def,evaluate_def,state_component_equality]>>
+  TRY
+    (ntac 2 (pop_assum mp_tac)>>fs[inst_def,assign_def,word_exp_def,get_vars_def,get_var_def,set_vars_def,alist_insert_def]>>
+    EVERY_CASE_TAC >>
+    fs[LET_THM,alist_insert_def,distinct_tar_reg_def,word_exp_def,lookup_insert,set_var_def,insert_shadow]>>NO_TAC)
+  >-
+    (ntac 2 (pop_assum mp_tac)>>LET_ELIM_TAC>>fs[distinct_tar_reg_def]>>
+    Cases_on`res'' = SOME Error`>>fs[]>>res_tac>>
+    EVERY_CASE_TAC>>fs[]>>
+    metis_tac[])
+  >-
+    (ntac 2 (pop_assum mp_tac)>>LET_ELIM_TAC>>fs[distinct_tar_reg_def]>>
+    unabbrev_all_tac>>
+    Cases_on`ret`>>Cases_on`handler`>>fs[evaluate_def]
+    >-
+      (EVERY_CASE_TAC>>fs[])
+    >-
+      (EVERY_CASE_TAC>>fs[]>>
+      res_tac>>fs[]>>
+      rfs[])
+    >>
+      PairCases_on`x`>>PairCases_on`x'`>>fs[]>>
+      Cases_on`get_vars args s`>>fs[]>>
+      Cases_on`find_code dest x s.code`>>fs[]>>
+      Cases_on`x'`>>Cases_on`cut_env x1 s.locals`>>fs[]>>
+      IF_CASES_TAC>>fs[push_env_def,LET_THM]>>
+      EVERY_CASE_TAC>>fs[]>>
+      res_tac>>fs[]>>
+      rfs[]))
+
+(*Syntactic correctness*)
+val three_to_two_reg_syn = prove(``
+  ∀prog. two_reg_insts (three_to_two_reg prog)``,
+  ho_match_mp_tac three_to_two_reg_ind>>rw[]>>fs[two_reg_insts_def,three_to_two_reg_def,LET_THM]>>EVERY_CASE_TAC>>fs[])
+
     
 (*No expressions nesting*)
 val flat_exp_conventions_def = Define`
